comments

AVM/Program.lean
@@ -5,35 +5,42 @@ import AVM.Program.Parameters
 
 namespace AVM
 
+/-- Representation of AVM programs. These are compiled to Anoma programs. -/
 inductive Program.{u} (lab : Ecosystem.Label) (ReturnType : Type u) : Type (u + 1) where
-  | constructor
+  | /-- Constructor call. -/
+    constructor
     (cid : lab.ClassId)
     (constrId : cid.label.ConstructorId)
     (args : constrId.Args.type)
     (next : ObjectId → Program lab ReturnType)
     : Program lab ReturnType
-  | destructor
+  | /-- Destructor call. -/
+    destructor
     (cid : lab.ClassId)
     (destrId : cid.label.DestructorId)
     (selfId : ObjectId)
     (args : destrId.Args.type)
     (next : Program lab ReturnType)
     : Program lab ReturnType
-  | method
+  | /-- Method call. -/
+    method
     (cid : lab.ClassId)
     (methodId : cid.label.MethodId)
     (selfId : ObjectId)
     (args : methodId.Args.type)
     (next : Program lab ReturnType)
     : Program lab ReturnType
-  | fetch
+  | /-- Object fetch by object id. -/
+    fetch
     (objId : TypedObjectId)
     (next : Object objId.classLabel → Program lab ReturnType)
     : Program lab ReturnType
-  | return
+  | /-- Return value. -/
+    return
     (val : ReturnType)
     : Program lab ReturnType
 
+/-- Program composition: invoke a program and then continue with another program. -/
 def Program.invoke
     {α β : Type u}
     {lab : Ecosystem.Label}
@@ -52,6 +59,11 @@ def Program.invoke
   | .return val =>
     next val
 
+/-- Parameters (generated random values and fetched obejcts) of the program,
+  *not* including the parameters of the sub-programs (the bodies of called
+  methods, constructors, destructors). In general, values of type
+  `prog.params.Product` are assumed to be adjusted (see
+  `Program.Parameters.Product`). -/
 def Program.params {lab : Ecosystem.Label} {α : Type u} (prog : Program lab α) : Parameters :=
   match prog with
   | .constructor _ _ _ next => .genId (fun newId => next newId |>.params)
@@ -60,6 +72,8 @@ def Program.params {lab : Ecosystem.Label} {α : Type u} (prog : Program lab α)
   | .fetch objId next => .fetch objId (fun obj => next obj |>.params)
   | .return _ => .empty
 
+/-- The return value of a program. The `vals` provided need to be adjusted (see
+  `Program.Parameters.Product`). -/
 def Program.value {lab : Ecosystem.Label} {α : Type u} (prog : Program lab α) (vals : prog.params.Product) : α :=
   match prog with
   | .constructor _ _ _ next =>
