AVM/Program/Translation.lean
@@ -5,4 +5,4 @@ import AVM.Task.Translation
 namespace AVM
 
 def Program.compile {lab : Ecosystem.Label} (eco : Ecosystem lab) (prog : Program lab Unit) : Anoma.Program :=
-  Class.Body.tasks eco prog |> Tasks.compose |>.toProgram
+  Class.Member.Body.tasks eco prog |> Tasks.compose |>.toProgram
