AVM/Tasks.lean
@@ -2,16 +2,29 @@ import AVM.Task
 
 namespace AVM
 
+/-- Tasks resulting from the compilation of an AVM program. The `Tasks` type
+  mimics more closely the structure of AVM programs than a single `Task`.
+  `AVM.Program` is compiled to `Tasks` which are then composed into a single
+  `Task`. The composition of `Tasks` collects and lifts out the parameters of
+  all subtasks. -/
 inductive Tasks (α : Type u) where
+  /-- Execute a subtask and continue. The `rest` continuation receives the
+    unadjusted parameter values. -/
   | task (task : Task) (rest : task.params.Product → Tasks α) : Tasks α
-  /-- The `rest` continuation receives the unadjusted original object value and
-    is supposed to adjust it by the modifications to that object that occurred
-    from the start of the program up to the fetch. -/
+  /-- Fetch an object and continue. The `rest` continuation receives the
+    unadjusted original object value and is supposed to adjust it by the
+    modifications to that object that occurred from the start of the program up
+    to the fetch. -/
   | fetch (param : TypedObjectId) (rest : Object param.classLabel → Tasks α) : Tasks α
   | rand (rest : Nat → Tasks α) : Tasks α
   | result (value : α) : Tasks α
   deriving Inhabited
 
+/-- `Tasks.params` includes the parameters of the sub-tasks, in contrast to
+  `Program.params` which doesn't include the parameters of the sub-programs. In
+  general, values in `tasks.params.Product` are assumed to be unadjusted (see
+  `Program.Parameters.Product`), in contrast to values in `prog.params.Product`
+  which are assumed to be adjusted. -/
 def Tasks.params {α} (tasks : Tasks α) : Program.Parameters :=
   match tasks with
   | .task t rest => (t.params.append (fun vals => (rest vals).params))
@@ -19,9 +32,10 @@ def Tasks.params {α} (tasks : Tasks α) : Program.Parameters :=
   | .rand rest => .rand (fun r => (rest r).params)
   | .result _ => .empty
 
-/-- `vals` are the object values as fetched from Anoma before the transaction
-  submission, i.e., they are not adjusted by subsequent modifications in the
-  program. -/
+/-- The return value of the tasks. `vals` are unadjusted parameter values (see
+  `Program.Parameters.Product`): the object values as fetched from Anoma at the
+  start of program execution, i.e., they are not adjusted by subsequent
+  modifications to these objects in the program. -/
 def Tasks.value {α} (tasks : Tasks α) (vals : tasks.params.Product) : α :=
   match tasks with
   | .task _ rest =>
